Added a new Examples file with the Zolotarev-Frobenius characterization of the Jacobi symbol (for odd modulus) as the sign of the permutation induced by multiplication modulo.
Also added a large number of miscellaneous results about integers
(more on primitive roots, quadratic residues and the Euler totient
function as well as the "minimal" operation on natural numbers) and
about permutations (isomorphic transfer, restriction, products, cyclic
permutations), quite a few in support of the Zolotarev proof but some
quite independent, e.g. Arazi's inversion formula for modular
inverses, INVERSE_MOD_INVERSION. Complete list of new definitions:

        zolotarev
        zolotarevu

and theorems:

        CHINESE_REMAINDER_USUAL
        DIVIDES_DIV_DIVIDES
        DIVIDES_DIV_SELF
        DIV_BY_DIV
        EVENPERM_CYCLIC
        EVENPERM_CYCLIC_N
        EVENPERM_ID
        EVENPERM_TRANSFER
        EVEN_MOD_EVEN
        GCD_2_CASES
        GCD_PRIME_CASES
        INDUCT_COPRIME_ALT
        INT_2_DIVIDES_ADD
        INT_2_DIVIDES_MUL
        INT_2_DIVIDES_POW
        INT_2_DIVIDES_SUB
        INVERSE_MOD_BOUND_LE
        INVERSE_MOD_INVERSION
        INVERSE_MOD_NONZERO
        INVERSE_MOD_NONZERO_ALT
        JACOBI_EQ_ZOLOTAREV
        JACOBI_EQ_ZOLOTAREV_PRIMEPOW
        LE_MINIMAL
        MINIMAL_LBOUND
        MINIMAL_LE
        MINIMAL_UBOUND
        MINIMAL_UNIQUE
        MOD_EVEN_2
        ODD_MOD_EVEN
        ORDER_LE_PHI
        PERMUTATION_CYCLIC
        PERMUTATION_CYCLIC_N
        PERMUTATION_RESTRICT
        PERMUTATION_ZOLOTAREV
        PERMUTATION_ZOLOTAREVU
        PERMUTES_ALT
        PERMUTES_CARTESIAN_PRODUCT
        PERMUTES_CYCLIC
        PERMUTES_CYCLIC_N
        PERMUTES_INDUCT_STRONG
        PERMUTES_INVERSE_FUNCTION
        PERMUTES_RESTRICT
        PERMUTES_RESTRICT_SET
        PERMUTES_TRANSFER
        PERMUTES_TRANSFER_BIJECTIONS
        PERMUTES_ZOLOTAREV
        PERMUTES_ZOLOTAREVU
        PERMUTES_ZOLOTAREV_ALT
        PHI_EQ_PRIME
        PHI_LIMIT_COMPOSITE
        POWER_RESIDUE_MODULO_PRIMITIVE_POWER
        PRIMITIVE_ROOT_IMAGE
        PRIMITIVE_ROOT_IMAGE_PRIME
        PRIMITIVE_ROOT_IMP_COPPRIME
        PRIMITIVE_ROOT_IMP_PRIME
        PRIMITIVE_ROOT_SURJECTIVE
        PRIMITIVE_ROOT_SURJECTIVE_ALT
        PRIMITIVE_ROOT_SURJECTIVE_PRIME
        PRIMITIVE_ROOT_SURJECTIVE_PRIME_ALT
        QUADRATIC_RESIDUE_MODULO_POWER_2
        QUADRATIC_RESIDUE_MODULO_POWER_2_STABLE
        QUADRATIC_RESIDUE_MODULO_PRIMITIVE_POWER
        SIGN_CARTESIAN_PRODUCT
        SIGN_CYCLIC
        SIGN_CYCLIC
        SIGN_ID
        SIGN_TRANSFER
        ZOLATAREVU_MOD
        ZOLATAREV_EQ_ZOLATAREVU
        ZOLATAREV_MOD
        ZOLOTAREVU_PRIMITIVE
        ZOLOTAREV_1
        ZOLOTAREV_CONG

Library/words.ml
@@ -304,9 +304,7 @@ let ODD_MOD_POW2 = prove
  (`!n k. ODD(n MOD 2 EXP k) <=> ~(k = 0) /\ ODD n`,
   REPEAT GEN_TAC THEN ASM_CASES_TAC `k = 0` THEN
   ASM_REWRITE_TAC[MOD_1; EXP; ODD] THEN
-  REWRITE_TAC[MESON[ODD_MOD; EXP_1] `ODD n <=> n MOD (2 EXP 1) = 1`] THEN
-  REWRITE_TAC[MOD_MOD_EXP_MIN] THEN
-  ASM_SIMP_TAC[ARITH_RULE `~(k = 0) ==> MIN k 1 = 1`]);;
+  ASM_SIMP_TAC[ODD_MOD_EVEN; EVEN_EXP; ARITH]);;
 
 let BINARY_DIGITSUM_BOUND = prove
  (`!b k. nsum {i | i < k} (\i. 2 EXP i * bitval(b i)) < 2 EXP k`,
@@ -729,6 +727,26 @@ let VAL_MOD_STEP = prove
   REWRITE_TAC[VAL_MOD; ARITH_RULE `i < k + 1 <=> i = k \/ i < k`] THEN
   REWRITE_TAC[SET_RULE `{x | x = a \/ P x} = a INSERT {x | P x}`] THEN
   SIMP_TAC[NSUM_CLAUSES; FINITE_NUMSEG_LT; IN_ELIM_THM; LT_REFL]);;
+
+let VAL_DIV = prove
+ (`!(x:N word) k.
+        val x DIV 2 EXP k =
+        nsum {i | k <= i /\ i < dimindex(:N)}
+             (\i. 2 EXP (i - k) * bitval(bit i x))`,
+  REPEAT GEN_TAC THEN REWRITE_TAC[val_def] THEN
+  SIMP_TAC[BINARY_DIGITSUM_DIV; FINITE_NUMSEG_LT] THEN
+  REWRITE_TAC[IN_ELIM_THM] THEN REWRITE_TAC[CONJ_SYM]);;
+
+let VAL_DIV_ALT = prove
+ (`!(x:N word) k.
+        val x DIV 2 EXP k =
+        nsum {i | i < dimindex(:N) - k}
+             (\i. 2 EXP i * bitval(bit (i + k) x))`,
+  REPEAT GEN_TAC THEN REWRITE_TAC[VAL_DIV] THEN
+  MATCH_MP_TAC NSUM_EQ_GENERAL_INVERSES THEN
+  EXISTS_TAC `\i:num. i - k` THEN
+  EXISTS_TAC `\i:num. i + k` THEN
+  SIMP_TAC[IN_ELIM_THM; SUB_ADD] THEN ARITH_TAC);;
 
 (* ------------------------------------------------------------------------- *)
 (* Corresponding signed 2s-complement mappings to and from integers.         *)
@@ -3068,6 +3086,296 @@ let WORD_BITMASK = prove
   REWRITE_TAC[EXP_EQ_0; ARITH_EQ]);;
 
 (* ------------------------------------------------------------------------- *)
+(* Trailing and leading zero count (returning word size for zero input).     *)
+(* ------------------------------------------------------------------------- *)
+
+let word_ctz = new_definition
+ `word_ctz (a:N word) =
+        if a = word 0 then dimindex(:N) else minimal i. bit i a`;;
+
+let word_clz = new_definition
+ `word_clz (a:N word) = dimindex(:N) - minimal m. !i. m <= i ==> ~bit i a`;;
+
+let WORD_CTZ_0 = prove
+ (`word_ctz(word 0:N word) = dimindex(:N)`,
+  REWRITE_TAC[word_ctz]);;
+
+let WORD_LE_CTZ = prove
+ (`!(a:N word) n.
+        n <= word_ctz a <=> n <= dimindex(:N) /\ !i. bit i a ==> n <= i`,
+  REPEAT GEN_TAC THEN REWRITE_TAC[word_ctz] THEN
+  COND_CASES_TAC THEN ASM_REWRITE_TAC[BIT_WORD_0] THEN
+  RULE_ASSUM_TAC(REWRITE_RULE[WORD_EQ_BITS_ALT; BIT_WORD_0]) THEN
+  W(MP_TAC o PART_MATCH (lhand o rand) LE_MINIMAL o lhand o snd) THEN
+  ANTS_TAC THENL [ASM_MESON_TAC[]; DISCH_THEN SUBST1_TAC] THEN
+  ASM_MESON_TAC[NOT_LE; LE_CASES; LE_TRANS]);;
+
+let WORD_CTZ_LE = prove
+ (`!(a:N word) n.
+        word_ctz a <= n <=> n < dimindex(:N) ==> ?i. i <= n /\ bit i a`,
+  REPEAT GEN_TAC THEN
+  GEN_REWRITE_TAC LAND_CONV [ARITH_RULE `m <= n <=> ~(SUC n <= m)`] THEN
+  REWRITE_TAC[WORD_LE_CTZ; DE_MORGAN_THM] THEN
+  REWRITE_TAC[ARITH_RULE `SUC n <= m <=> ~(m <= n)`] THEN
+  MESON_TAC[NOT_LT]);;
+
+let WORD_CTZ_LE_DIMINDEX = prove
+ (`!a:N word. word_ctz(a) <= dimindex(:N)`,
+  REWRITE_TAC[WORD_CTZ_LE; LT_REFL]);;
+
+let WORD_CTZ_LBOUND = prove
+ (`!(a:N word) i. bit i a ==> word_ctz(a) <= i`,
+  REWRITE_TAC[WORD_CTZ_LE] THEN MESON_TAC[LE_REFL]);;
+
+let WORD_CTZ_EQ_DIMINDEX = prove
+ (`!a:N word. word_ctz a = dimindex(:N) <=> a = word 0`,
+  REWRITE_TAC[GSYM LE_ANTISYM; WORD_CTZ_LE_DIMINDEX; WORD_LE_CTZ] THEN
+  REWRITE_TAC[LE_REFL; WORD_EQ_BITS_ALT; BIT_WORD_0] THEN MESON_TAC[NOT_LE]);;
+
+let WORD_CTZ_LT_DIMINDEX = prove
+ (`!a:N word. word_ctz a < dimindex(:N) <=> ~(a = word 0)`,
+  REWRITE_TAC[LT_LE; WORD_CTZ_LE_DIMINDEX; WORD_CTZ_EQ_DIMINDEX]);;
+
+let WORD_CTZ_EQ_0 = prove
+ (`!a:N word. word_ctz a = 0 <=> bit 0 a`,
+  REWRITE_TAC[GSYM(CONJUNCT1 LE)] THEN
+  REWRITE_TAC[WORD_CTZ_LE; CONJUNCT1 LE; UNWIND_THM2] THEN
+  SIMP_TAC[DIMINDEX_GE_1; LE_1]);;
+
+let WORD_CTZ_UNIQUE_GEN = prove
+ (`!(a:N word) n.
+        word_ctz a = n <=>
+        n <= dimindex(:N) /\
+        (n < dimindex(:N) ==> bit n a) /\
+        (!i. i < n ==> ~bit i a)`,
+  REPEAT GEN_TAC THEN GEN_REWRITE_TAC LAND_CONV [GSYM LE_ANTISYM] THEN
+  REWRITE_TAC[WORD_CTZ_LE; WORD_LE_CTZ] THEN
+  ASM_CASES_TAC `n <= dimindex(:N)` THEN ASM_REWRITE_TAC[] THEN
+  REWRITE_TAC[NOT_LT; MESON[] `p ==> ~bit a b <=> bit a b ==> ~p`] THEN
+  ASM_CASES_TAC `n < dimindex(:N)` THEN ASM_REWRITE_TAC[] THEN
+  MESON_TAC[LE_ANTISYM]);;
+
+let WORD_CTZ_UNIQUE = prove
+ (`!(a:N word) n.
+        n < dimindex(:N)
+        ==> (word_ctz a = n <=> bit n a /\ !i. i < n ==> ~bit i a)`,
+  SIMP_TAC[WORD_CTZ_UNIQUE_GEN; LT_IMP_LE]);;
+
+let WORD_LE_CTZ_VAL_MOD = prove
+ (`!(a:N word) n.
+        n <= word_ctz a <=>
+        n <= dimindex(:N) /\ val a MOD 2 EXP n = 0`,
+  REPEAT GEN_TAC THEN REWRITE_TAC[WORD_LE_CTZ] THEN
+  ASM_CASES_TAC `n <= dimindex(:N)` THEN ASM_REWRITE_TAC[] THEN
+  GEN_REWRITE_TAC (LAND_CONV o ONCE_DEPTH_CONV) [GSYM CONTRAPOS_THM] THEN
+  REWRITE_TAC[VAL_MOD; NOT_LE] THEN
+  SIMP_TAC[NSUM_EQ_0_IFF; FINITE_NUMSEG_LT; IN_ELIM_THM] THEN
+  REWRITE_TAC[MULT_EQ_0; EXP_EQ_0; ARITH_EQ; BITVAL_EQ_0]);;
+
+let WORD_LE_CTZ_VAL = prove
+ (`!(a:N word) n.
+        n <= word_ctz a <=>
+        n <= dimindex(:N) /\ 2 EXP n divides val a`,
+  REWRITE_TAC[WORD_LE_CTZ_VAL_MOD] THEN
+  MESON_TAC[divides; MOD_EQ_0; MULT_SYM]);;
+
+let WORD_CTZ_UNIQUE_VAL = prove
+ (`!(a:N word) n.
+        val a MOD (2 EXP (n + 1)) = 2 EXP n
+        ==> word_ctz a = n`,
+  REPEAT STRIP_TAC THEN FIRST_ASSUM(MP_TAC o SPEC `dimindex(:N)` o MATCH_MP
+   (ARITH_RULE `a MOD p = n
+                ==> !e. a MOD p <= a ==> a < 2 EXP e ==> n < 2 EXP e`)) THEN
+  REWRITE_TAC[VAL_BOUND; MOD_LE; LT_EXP; ARITH] THEN
+  DISCH_TAC THEN ASM_SIMP_TAC[WORD_CTZ_UNIQUE] THEN
+  CONJ_TAC THENL [ASM_REWRITE_TAC[BIT_VAL_MOD; LE_REFL]; ALL_TAC] THEN
+  FIRST_X_ASSUM(MP_TAC o AP_TERM `\x. x MOD (2 EXP n)`) THEN
+  REWRITE_TAC[EXP_ADD; MOD_MOD; MOD_REFL] THEN
+  REWRITE_TAC[GSYM VAL_WORD_AND_MASK] THEN
+  REWRITE_TAC[VAL_EQ_0; WORD_EQ_BITS; BIT_WORD_0] THEN
+  REWRITE_TAC[BIT_WORD_AND; BIT_WORD_OF_BITS; IN_ELIM_THM] THEN
+  ASM_MESON_TAC[LT_TRANS]);;
+
+let WORD_CLZ_0 = prove
+ (`word_clz(word 0:N word) = dimindex(:N)`,
+  REWRITE_TAC[word_clz; BIT_WORD_0] THEN
+  MATCH_MP_TAC(ARITH_RULE `d = 0 ==> m - d = m`) THEN
+  MATCH_MP_TAC MINIMAL_UNIQUE THEN REWRITE_TAC[LT]);;
+
+let WORD_SIZE_SUB_CLZ = prove
+ (`!(a:N word).
+        dimindex(:N) - word_clz(a) = (minimal m. !i. m <= i ==> ~bit i a)`,
+  REPEAT GEN_TAC THEN REWRITE_TAC[word_clz] THEN
+  MATCH_MP_TAC(ARITH_RULE `m:num <= n ==> n - (n - m) = m`) THEN
+  MATCH_MP_TAC MINIMAL_UBOUND THEN MESON_TAC[BIT_TRIVIAL]);;
+
+let WORD_CLZ_LE_DIMINDEX = prove
+ (`!a:N word. word_clz(a) <= dimindex(:N)`,
+  REWRITE_TAC[word_clz] THEN ARITH_TAC);;
+
+let WORD_LE_CLZ = prove
+ (`!(a:N word) n.
+        n <= word_clz(a) <=>
+        n <= dimindex(:N) /\ !i. bit i a ==> i + n < dimindex(:N)`,
+  REPEAT GEN_TAC THEN ASM_CASES_TAC `n <= dimindex(:N)` THENL
+   [ASM_REWRITE_TAC[]; ASM_MESON_TAC[WORD_CLZ_LE_DIMINDEX; LE_TRANS]] THEN
+  TRANS_TAC EQ_TRANS
+   `dimindex(:N) - word_clz(a:N word) <= dimindex(:N) - n` THEN
+  CONJ_TAC THENL [ASM_ARITH_TAC; REWRITE_TAC[WORD_SIZE_SUB_CLZ]] THEN
+  W(MP_TAC o PART_MATCH (lhand o rand) MINIMAL_LE o lhand o snd) THEN
+  REWRITE_TAC[] THEN ANTS_TAC THENL
+   [MESON_TAC[BIT_TRIVIAL]; DISCH_THEN SUBST1_TAC] THEN
+  ONCE_REWRITE_TAC[TAUT `p ==> ~q <=> q ==> ~p`] THEN
+  REWRITE_TAC[NOT_LE; MESON[LE_REFL; LTE_TRANS]
+   `(?m:num. m <= n /\ !i. P i ==> i < m) <=> (!i. P i ==> i < n)`] THEN
+  ASM_SIMP_TAC[ARITH_RULE `n:num <= d ==> (i < d - n <=> i + n < d)`]);;
+
+let WORD_CLZ_LE = prove
+ (`!(a:N word) n.
+        word_clz(a) <= n <=>
+        n < dimindex(:N) ==> ?i. dimindex(:N) <= i + n + 1 /\ bit i a`,
+  REPEAT GEN_TAC THEN
+  GEN_REWRITE_TAC LAND_CONV [ARITH_RULE `m <= n <=> ~(SUC n <= m)`] THEN
+  REWRITE_TAC[WORD_LE_CLZ; DE_MORGAN_THM] THEN REWRITE_TAC[LE_SUC_LT] THEN
+  ASM_CASES_TAC `n < dimindex(:N)` THEN ASM_REWRITE_TAC[] THEN
+  REWRITE_TAC[NOT_FORALL_THM; NOT_IMP; NOT_LT] THEN
+  MESON_TAC[ARITH_RULE `i + SUC n = i + n + 1`]);;
+
+let WORD_CLZ_LBOUND_ALT = prove
+ (`!(a:N word) i. bit i a ==> word_clz(a) + i < dimindex(:N)`,
+  REPEAT STRIP_TAC THEN MATCH_MP_TAC(ARITH_RULE
+   `~(n <= i) /\ c <= (n - 1) - i ==> c + i < n`) THEN
+  CONJ_TAC THENL [ASM_MESON_TAC[BIT_TRIVIAL]; ALL_TAC] THEN
+  REWRITE_TAC[WORD_CLZ_LE] THEN REPEAT STRIP_TAC THEN EXISTS_TAC `i:num` THEN
+  ASM_REWRITE_TAC[] THEN ASM_ARITH_TAC);;
+
+let WORD_CLZ_LBOUND = prove
+ (`!(a:N word) i. bit i a ==> word_clz(a) < dimindex(:N) - i`,
+  MESON_TAC[WORD_CLZ_LBOUND_ALT; ARITH_RULE `a + i:num < n ==> a < n - i`]);;
+
+let WORD_CLZ_EQ_DIMINDEX = prove
+ (`!a:N word. word_clz a = dimindex(:N) <=> a = word 0`,
+  REWRITE_TAC[GSYM LE_ANTISYM; WORD_CLZ_LE_DIMINDEX; WORD_LE_CLZ] THEN
+  REWRITE_TAC[LE_REFL; ARITH_RULE `~(i + n:num < n)`] THEN
+  REWRITE_TAC[WORD_EQ_BITS; BIT_WORD_0]);;
+
+let WORD_CLZ_LT_DIMINDEX = prove
+ (`!a:N word. word_clz a < dimindex(:N) <=> ~(a = word 0)`,
+  REWRITE_TAC[LT_LE; WORD_CLZ_LE_DIMINDEX; WORD_CLZ_EQ_DIMINDEX]);;
+
+let WORD_CLZ_EQ_0 = prove
+ (`!a:N word. word_clz a = 0 <=> bit (dimindex(:N) - 1) a`,
+  REWRITE_TAC[GSYM(CONJUNCT1 LE)] THEN
+  REWRITE_TAC[WORD_CLZ_LE; CONJUNCT1 LE; UNWIND_THM2] THEN
+  GEN_TAC THEN SIMP_TAC[DIMINDEX_GE_1; LE_1; ADD_CLAUSES] THEN
+  GEN_REWRITE_TAC (LAND_CONV o ONCE_DEPTH_CONV) [MESON[BIT_TRIVIAL]
+   `bit i (a:N word) <=> ~(dimindex(:N) <= i) /\ bit i a`] THEN
+  REWRITE_TAC[CONJ_ASSOC; DIMINDEX_GE_1; UNWIND_THM2; ARITH_RULE
+   `n <= i + 1 /\ ~(n <= i) <=> i = n - 1 /\ 1 <= n`]);;
+
+let WORD_CLZ_DECOMP = prove
+ (`!a:N word.
+        word_clz(a) + (minimal m. !i. m <= i ==> ~bit i a) = dimindex(:N)`,
+  GEN_TAC THEN REWRITE_TAC[word_clz] THEN
+  MATCH_MP_TAC SUB_ADD THEN MATCH_MP_TAC MINIMAL_UBOUND THEN
+  MESON_TAC[BIT_TRIVIAL]);;
+
+let WORD_CLZ_UNIQUE_GEN = prove
+ (`!(a:N word) n.
+        word_clz a = n <=>
+        n <= dimindex(:N) /\
+        (n < dimindex(:N) ==> bit (dimindex(:N) - n - 1) a) /\
+        (!i. dimindex(:N) - n <= i ==> ~bit i a)`,
+  REPEAT GEN_TAC THEN GEN_REWRITE_TAC LAND_CONV [GSYM LE_ANTISYM] THEN
+  REWRITE_TAC[WORD_CLZ_LE; WORD_LE_CLZ] THEN
+  ASM_CASES_TAC `n <= dimindex(:N)` THEN ASM_REWRITE_TAC[] THEN
+  REWRITE_TAC[NOT_LT; MESON[] `p ==> ~bit a b <=> bit a b ==> ~p`] THEN
+  ASM_SIMP_TAC[ARITH_RULE `n:num <= N ==> (~(N - n <= i) <=> i + n < N)`] THEN
+  ASM_CASES_TAC `n < dimindex(:N)` THEN ASM_REWRITE_TAC[] THEN
+  MATCH_MP_TAC(TAUT `(r ==> (p <=> q)) ==> (p /\ r <=> q /\ r)`) THEN
+  DISCH_THEN(fun th -> ONCE_REWRITE_TAC[MATCH_MP
+   (MESON[] `(!i. bit i a ==> P i)
+             ==> (!i. bit i a <=> P i /\ bit i a)`) th]) THEN
+  ASM_REWRITE_TAC[CONJ_ASSOC; DIMINDEX_GE_1; UNWIND_THM2; ARITH_RULE
+   `N <= i + n + 1 /\ i + n < N <=> 1 <= N /\ n < N /\ i = N - n - 1`] THEN
+  EQ_TAC THEN SIMP_TAC[] THEN ASM_ARITH_TAC);;
+
+let WORD_CLZ_UNIQUE = prove
+ (`!(a:N word) n.
+        n < dimindex(:N)
+        ==> (word_clz a = n <=>
+             bit (dimindex(:N) - n - 1) a /\
+             !i. dimindex(:N) - n <= i ==> ~bit i a)`,
+  SIMP_TAC[WORD_CLZ_UNIQUE_GEN; LT_IMP_LE]);;
+
+let WORD_LE_CLZ_VAL = prove
+ (`!(a:N word) n.
+        n <= word_clz a <=>
+        n <= dimindex(:N) /\ val a < 2 EXP (dimindex(:N) - n)`,
+  REPEAT GEN_TAC THEN REWRITE_TAC[WORD_LE_CLZ] THEN
+  ASM_CASES_TAC `n <= dimindex(:N)` THEN ASM_REWRITE_TAC[] THEN
+  TRANS_TAC EQ_TRANS `val(a:N word) DIV 2 EXP (dimindex(:N) - n) = 0` THEN
+  CONJ_TAC THENL [ALL_TAC; SIMP_TAC[DIV_EQ_0; EXP_EQ_0; ARITH_EQ]] THEN
+  REWRITE_TAC[VAL_DIV] THEN
+  W(MP_TAC o PART_MATCH (lhand o rand) NSUM_EQ_0_IFF o rand o snd) THEN
+  ANTS_TAC THENL
+   [MATCH_MP_TAC FINITE_SUBSET THEN EXISTS_TAC `{i | i < dimindex(:N)}` THEN
+    REWRITE_TAC[FINITE_NUMSEG_LT] THEN SET_TAC[];
+    DISCH_THEN SUBST1_TAC] THEN
+  REWRITE_TAC[FORALL_IN_GSPEC; MULT_EQ_0; EXP_EQ_0; ARITH_EQ; BITVAL_EQ_0] THEN
+  ASSUME_TAC(SPEC `a:N word` BIT_TRIVIAL) THEN
+  EQ_TAC THEN MATCH_MP_TAC MONO_FORALL THEN X_GEN_TAC `i:num` THEN
+  FIRST_X_ASSUM(MP_TAC o SPEC `i:num`) THEN
+  ASM_CASES_TAC `bit i (a:N word)` THEN ASM_REWRITE_TAC[] THEN
+  ASM_ARITH_TAC);;
+
+let WORD_LE_CLZ_VAL_MULT = prove
+ (`!(a:N word) n.
+        n <= word_clz a <=>
+        n <= dimindex(:N) /\ 2 EXP n * val a < 2 EXP dimindex(:N)`,
+  REPEAT GEN_TAC THEN REWRITE_TAC[WORD_LE_CLZ_VAL] THEN
+  ASM_CASES_TAC `n <= dimindex(:N)` THEN ASM_REWRITE_TAC[] THEN
+  SUBGOAL_THEN `2 EXP dimindex(:N) = 2 EXP n * 2 EXP (dimindex(:N) - n)`
+  SUBST1_TAC THENL
+   [REWRITE_TAC[GSYM EXP_ADD] THEN AP_TERM_TAC THEN ASM_ARITH_TAC;
+    REWRITE_TAC[LT_MULT_LCANCEL; EXP_EQ_0; ARITH_EQ]]);;
+
+let WORD_LE_CLZ_VAL_DIV = prove
+ (`!(a:N word) n.
+        n <= word_clz a <=>
+        n <= dimindex(:N) /\ val a DIV (2 EXP (dimindex(:N) - n)) = 0`,
+  SIMP_TAC[DIV_EQ_0; EXP_EQ_0; ARITH_EQ; WORD_LE_CLZ_VAL]);;
+
+let VAL_BOUND_CLZ = prove
+ (`!(a:N word) n.
+        2 EXP n * val a < 2 EXP dimindex(:N) <=>
+        a = word 0 \/ n <= word_clz a`,
+  REPEAT GEN_TAC THEN ASM_CASES_TAC `a:N word = word 0` THEN
+  ASM_REWRITE_TAC[VAL_WORD_0; MULT_CLAUSES; EXP_LT_0; EXP_EQ_0; ARITH_EQ] THEN
+  REWRITE_TAC[WORD_LE_CLZ_VAL_MULT] THEN
+  REWRITE_TAC[TAUT `(p <=> q /\ p) <=> p ==> q`] THEN
+  DISCH_THEN(MP_TAC o MATCH_MP (ARITH_RULE
+   `n * a < N ==> n * 1 <= n * a ==> n <= N`)) THEN
+  REWRITE_TAC[LE_EXP; ARITH_EQ; EXP_EQ_0; LE_MULT_LCANCEL] THEN
+  ASM_SIMP_TAC[LE_1; VAL_EQ_0]);;
+
+let WORD_CLZ_UNIQUE_VAL = prove
+ (`!(a:N word) n.
+        n < dimindex(:N) /\
+        val a DIV (2 EXP (dimindex(:N) - n - 1)) = 1
+        ==> word_clz a = n`,
+  REPEAT STRIP_TAC THEN ASM_SIMP_TAC[WORD_CLZ_UNIQUE] THEN
+  CONJ_TAC THENL [ASM_REWRITE_TAC[BIT_VAL; ARITH]; ALL_TAC] THEN
+  X_GEN_TAC `i:num` THEN DISCH_TAC THEN
+  SUBGOAL_THEN `i = (dimindex (:N) - n - 1) + SUC(i - (dimindex(:N) - n))`
+  SUBST1_TAC THENL [ASM_ARITH_TAC; ALL_TAC] THEN
+  ASM_SIMP_TAC[BIT_VAL; EXP_ADD; GSYM DIV_DIV] THEN
+  MATCH_MP_TAC(MESON[ODD] `n = 0 ==> ~ODD n`) THEN
+  SIMP_TAC[DIV_EQ_0; ARITH_EQ; EXP_EQ_0] THEN
+  GEN_REWRITE_TAC LAND_CONV [ARITH_RULE `1 = 2 EXP 0`] THEN
+  REWRITE_TAC[LT_EXP] THEN ARITH_TAC);;
+
+(* ------------------------------------------------------------------------- *)
 (* JVM-specific word operations, though they may well work in other places.  *)
 (*                                                                           *)
 (* All shift operations mask out the lower bits as the unsigned shift count. *)
@@ -4329,6 +4637,81 @@ let WORD_ODDPARITY_CONV =
       when is_numeral n -> conv tm
     | _ -> failwith "WORD_ODDPARITY_CONV");;
 
+let WORD_CTZ_CONV =
+  let ctz =
+    let rec ctza a n =
+      if mod_num n num_2 =/ num_0 then ctza (a + 1) (quo_num n num_2) else a in
+    fun n -> ctza 0 n
+  and pth_0 = prove
+    (`!(a:N word). val a = 0 ==> word_ctz a = dimindex(:N)`,
+     SIMP_TAC[VAL_EQ_0; WORD_CTZ_0])
+  and pth = prove
+   (`!(a:N word) v.
+        val a = v
+        ==> !n e. 2 EXP n = e /\ v MOD (2 * e) = e ==> word_ctz a = n`,
+    REPEAT GEN_TAC THEN DISCH_THEN(SUBST1_TAC o SYM) THEN REPEAT GEN_TAC THEN
+    REWRITE_TAC[IMP_CONJ] THEN DISCH_THEN(SUBST1_TAC o SYM) THEN
+    REWRITE_TAC[GSYM(CONJUNCT2 EXP); ADD1] THEN
+    REWRITE_TAC[WORD_CTZ_UNIQUE_VAL]) in
+  fun tm ->
+    match tm with
+      Comb(Const("word_ctz",_),Comb(Const("word",_),t))
+               when is_numeral t ->
+        let th1 = ISPEC (rand tm) pth in
+        let th2 = WORD_VAL_CONV(lhand(lhand(snd(dest_forall(concl th1))))) in
+        let mtm = rand(concl th2) in
+        let m = dest_numeral mtm in
+        if m =/ num_0 then
+          CONV_RULE (RAND_CONV(!word_SIZE_CONV)) (MATCH_MP pth_0 th2)
+        else
+          let th3 = MP (SPEC mtm th1) th2 in
+          let n = ctz m in
+          let th4 = SPECL [mk_small_numeral n; mk_numeral(pow2 n)] th3 in
+          MP th4 (EQT_ELIM(NUM_REDUCE_CONV(lhand(concl th4))))
+  | _ -> failwith "WORD_CTZ_CONV";;
+
+let WORD_CLZ_CONV =
+  let clz k =
+    let m = pow2 k in
+    let rec clza a n =
+      if n </ m then clza (a + 1) (num_2 */ n) else a in
+    fun n ->
+      if n =/ num_0 then k else min k (clza (-1) n)
+  and pth_0 = prove
+    (`!(a:N word). val a = 0 ==> word_clz a = dimindex(:N)`,
+     SIMP_TAC[VAL_EQ_0; WORD_CLZ_0])
+  and pth = prove
+   (`!(a:N word) v.
+        val a = v
+        ==> !n d. n + 1 + d = dimindex(:N) /\ v DIV (2 EXP d) = 1
+                  ==> word_clz a = n`,
+    REPEAT GEN_TAC THEN DISCH_THEN(SUBST1_TAC o SYM) THEN
+    REPEAT STRIP_TAC THEN MATCH_MP_TAC WORD_CLZ_UNIQUE_VAL THEN
+    CONJ_TAC THENL [ASM_ARITH_TAC; ALL_TAC] THEN
+    ASM_MESON_TAC[ARITH_RULE `n + 1 + d = N ==> N - n - 1 = d`]) in
+  fun tm ->
+    match tm with
+      Comb(Const("word_clz",_),Comb(Const("word",_),t))
+               when is_numeral t ->
+        let th1 = ISPEC (rand tm) pth in
+        let th2 = WORD_VAL_CONV(lhand(lhand(snd(dest_forall(concl th1))))) in
+        let mtm = rand(concl th2) in
+        let m = dest_numeral mtm in
+        if m =/ num_0 then
+          CONV_RULE (RAND_CONV(!word_SIZE_CONV)) (MATCH_MP pth_0 th2)
+        else
+          let th3 = MP (SPEC mtm th1) th2 in
+          let th4 = CONV_RULE
+           (BINDER_CONV(BINDER_CONV(LAND_CONV(LAND_CONV
+               (RAND_CONV(!word_SIZE_CONV)))))) th3 in
+          let btm = lhand(lhand(snd(strip_forall(concl th4)))) in
+          let e = dest_small_numeral(rand btm) in
+          let n = clz e m in
+          let d = e - (n + 1) in
+          let th5 = SPECL [mk_small_numeral n; mk_small_numeral d] th4 in
+          MP th5 (EQT_ELIM(NUM_REDUCE_CONV(lhand(concl th5))))
+  | _ -> failwith "WORD_CLZ_CONV";;
+
 let WORD_JSHL_CONV =
   let pth = prove
    (`word_jshl (word(NUMERAL m):N word) (word(NUMERAL n):N word) =
@@ -4435,6 +4818,8 @@ let WORD_RED_CONV =
     `word_popcount (word(NUMERAL n):N word)`,WORD_POPCOUNT_CONV;
     `word_evenparity (word(NUMERAL n):N word)`,WORD_EVENPARITY_CONV;
     `word_oddparity (word(NUMERAL n):N word)`,WORD_ODDPARITY_CONV;
+    `word_ctz (word(NUMERAL n):N word)`,WORD_CTZ_CONV;
+    `word_clz (word(NUMERAL n):N word)`,WORD_CLZ_CONV;
     `word_jshl (word(NUMERAL m):N word) (word(NUMERAL n))`,WORD_JSHL_CONV;
     `word_jshr (word(NUMERAL m):N word) (word(NUMERAL n))`,WORD_JSHR_CONV;
     `word_jushr (word(NUMERAL m):N word) (word(NUMERAL n))`,WORD_JUSHR_CONV;
