arith.ml
@@ -1278,6 +1278,10 @@ let MOD_MOD_LE = prove
   REPEAT STRIP_TAC THEN MATCH_MP_TAC MOD_LT THEN
   ASM_MESON_TAC[DIVISION; LTE_TRANS]);;
 
+let MOD_EVEN_2 = prove
+ (`!m n. EVEN n ==> m MOD n MOD 2 = m MOD 2`,
+  SIMP_TAC[EVEN_EXISTS; LEFT_IMP_EXISTS_THM; MOD_MOD]);;
+
 let DIV_MULT2 = prove
  (`!m n p. ~(m = 0) ==> ((m * n) DIV (m * p) = n DIV p)`,
   REPEAT STRIP_TAC THEN ASM_CASES_TAC `p = 0` THEN
@@ -1400,6 +1404,15 @@ let ODD_MOD = prove
 let MOD_2_CASES = prove
  (`!n. n MOD 2 = if EVEN n then 0 else 1`,
   MESON_TAC[EVEN_MOD; ODD_MOD; NOT_ODD]);;
+
+let EVEN_MOD_EVEN = prove
+ (`!m n. EVEN n ==> (EVEN(m MOD n) <=> EVEN m)`,
+  REPEAT STRIP_TAC THEN REWRITE_TAC[EVEN_MOD] THEN
+  ASM_SIMP_TAC[MOD_EVEN_2]);;
+
+let ODD_MOD_EVEN = prove
+ (`!m n. EVEN n ==> (ODD(m MOD n) <=> ODD m)`,
+  SIMP_TAC[GSYM NOT_EVEN; EVEN_MOD_EVEN]);;
 
 let MOD_MULT_RMOD = prove
  (`!m n p. (m * (p MOD n)) MOD n = (m * p) MOD n`,
@@ -1689,6 +1702,30 @@ let MINIMAL = prove
  (`!P. (?n. P n) <=> P((minimal) P) /\ (!m. m < (minimal) P ==> ~(P m))`,
   GEN_TAC THEN REWRITE_TAC[minimal] THEN CONV_TAC(RAND_CONV SELECT_CONV) THEN
   REWRITE_TAC[GSYM num_WOP]);;
+
+let MINIMAL_UNIQUE = prove
+ (`!P n. P n /\ (!m. m < n ==> ~P m) ==> (minimal) P = n`,
+  REPEAT STRIP_TAC THEN REWRITE_TAC[minimal] THEN
+  MATCH_MP_TAC SELECT_UNIQUE THEN ASM_MESON_TAC[LT_CASES]);;
+
+let LE_MINIMAL = prove
+ (`!P n.
+        (?r. P r) ==> (n <= (minimal) P <=> !i. P i ==> n <= i)`,
+  REPEAT GEN_TAC THEN GEN_REWRITE_TAC LAND_CONV [MINIMAL] THEN
+  MESON_TAC[NOT_LE; LE_TRANS]);;
+
+let MINIMAL_LE = prove
+ (`!P n. (?r. P r) ==> ((minimal) P <= n <=> ?i. i <= n /\ P i)`,
+  REWRITE_TAC[GSYM NOT_LT] THEN REWRITE_TAC[GSYM LE_SUC_LT] THEN
+  SIMP_TAC[LE_MINIMAL] THEN MESON_TAC[]);;
+
+let MINIMAL_UBOUND = prove
+ (`!P n. P n ==> (minimal) P <= n`,
+  MESON_TAC[MINIMAL; NOT_LT]);;
+
+let MINIMAL_LBOUND = prove
+ (`!P n. (?r. P r) /\ (!m. m < n ==> ~P m) ==> n <= (minimal) P`,
+  SIMP_TAC[LE_MINIMAL] THEN MESON_TAC[NOT_LT]);;
 
 (* ------------------------------------------------------------------------- *)
 (* A common lemma for transitive relations.                                  *)
